hax-lib/proof-libs/coq/coq/generated-core/src/Core_Base_Pos.v
@@ -9,413 +9,428 @@ Require Import String.
 Require Import Coq.Floats.Floats.
 From RecordUpdate Require Import RecordSet.
 Import RecordSetNotations.
+From Core Require Import Core.
 
-(* From Core Require Import Core. *)
+(* NotImplementedYet *)
 
-From Core Require Import Core_Base_Spec.
-Export Core_Base_Spec.
 
-From Core Require Import Core_Base_Binary.
-Export Core_Base_Binary.
 
-From Core Require Import Core_Cmp (t_Ordering).
-Export Core_Cmp (t_Ordering).
 
-Definition haxint_double (s : t_HaxInt) : t_HaxInt :=
-  match match_pos (s) with
-  | POS_ZERO =>
-    v_HaxInt_ZERO
-  | POS_POS (p) =>
-    positive_to_int (xO (p))
-  end.
 
-Definition haxint_shr__half (s : t_HaxInt) : t_HaxInt :=
-  match match_pos (s) with
-  | POS_ZERO =>
-    v_HaxInt_ZERO
-  | POS_POS (n) =>
-    match match_positive (n) with
-    | POSITIVE_XH =>
-      v_HaxInt_ZERO
-    | POSITIVE_XO (p) =>
-      positive_to_int (p)
-    | POSITIVE_XI (p) =>
-      positive_to_int (p)
+
+
+Inductive t_Mask : Type :=
+| Mask_IsPos : Core_Base_Spec_Binary_Positive.t_Positive -> _
+| Mask_IsNul
+| Mask_IsNeg.
+
+
+
+
+Definition haxint_cmp (lhs : Core_Base_Spec_Haxint.t_HaxInt) (rhs : Core_Base_Spec_Haxint.t_HaxInt) : Core_Cmp.t_Ordering :=
+  match Core_Base_Spec_Binary_Pos.match_pos (lhs) with
+  | Core_Base_Spec_Binary_Pos.POS_ZERO =>
+    match Core_Base_Spec_Binary_Pos.match_pos (rhs) with
+    | Core_Base_Spec_Binary_Pos.POS_ZERO =>
+      Core_Cmp.Ordering_Equal
+    | Core_Base_Spec_Binary_Pos.POS_POS (q) =>
+      Core_Cmp.Ordering_Less
+    end
+  | Core_Base_Spec_Binary_Pos.POS_POS (p) =>
+    match Core_Base_Spec_Binary_Pos.match_pos (rhs) with
+    | Core_Base_Spec_Binary_Pos.POS_ZERO =>
+      Core_Cmp.Ordering_Greater
+    | Core_Base_Spec_Binary_Pos.POS_POS (q) =>
+      Core_Base_Binary.positive_cmp (p) (q)
     end
   end.
 
-Definition haxint_sub__double_mask (lhs : t_HaxInt) : t_HaxInt :=
-  match match_pos (lhs) with
-  | POS_ZERO =>
-    v_HaxInt_ZERO
-  | POS_POS (p) =>
-    positive_to_int (xO (p))
+Definition haxint_lt (lhs : Core_Base_Spec_Haxint.t_HaxInt) (rhs : Core_Base_Spec_Haxint.t_HaxInt) : bool :=
+  match Core_Option.Option_Some (haxint_cmp (lhs) (rhs)) with
+  | Core_Option.Option_Some (Core_Cmp.Ordering_Less) =>
+    (true : bool)
+  | _ =>
+    (false : bool)
   end.
 
-Definition haxint_sub__succ_double_mask (lhs : t_HaxInt) : t_HaxInt :=
-  match match_pos (lhs) with
-  | POS_ZERO =>
-    positive_to_int (xH)
-  | POS_POS (p) =>
-    positive_to_int (xI (p))
+Definition haxint_le (lhs : Core_Base_Spec_Haxint.t_HaxInt) (rhs : Core_Base_Spec_Haxint.t_HaxInt) : bool :=
+  match Core_Option.Option_Some (haxint_cmp (lhs) (rhs)) with
+  | Core_Option.Option_Some (Core_Cmp.Ordering_Less
+  | Core_Cmp.Ordering_Equal) =>
+    (true : bool)
+  | _ =>
+    (false : bool)
   end.
 
-Definition haxint_succ_double (s : t_HaxInt) : t_Positive :=
-  match match_pos (s) with
-  | POS_ZERO =>
-    xH
-  | POS_POS (p) =>
-    xI (p)
-  end.
-
-Fixpoint bitand_binary (lhs : t_Positive) (rhs : t_Positive) : t_HaxInt :=
-  match match_positive (lhs) with
-  | POSITIVE_XH =>
-    match match_positive (rhs) with
-    | POSITIVE_XO (q) =>
-      v_HaxInt_ZERO
-    | POSITIVE_XI (_)
-    | POSITIVE_XH =>
-      v_HaxInt_ONE
+Definition haxint_add (lhs : Core_Base_Spec_Haxint.t_HaxInt) (rhs : Core_Base_Spec_Haxint.t_HaxInt) : Core_Base_Spec_Haxint.t_HaxInt :=
+  match Core_Base_Spec_Binary_Pos.match_pos (lhs) with
+  | Core_Base_Spec_Binary_Pos.POS_ZERO =>
+    rhs
+  | Core_Base_Spec_Binary_Pos.POS_POS (p) =>
+    match Core_Base_Spec_Binary_Pos.match_pos (rhs) with
+    | Core_Base_Spec_Binary_Pos.POS_ZERO =>
+      Core_Base_Spec_Binary_Positive.positive_to_int (p)
+    | Core_Base_Spec_Binary_Pos.POS_POS (q) =>
+      Core_Base_Spec_Binary_Positive.positive_to_int (Core_Base_Binary.positive_add (p) (q))
     end
-  | POSITIVE_XO (p) =>
-    match match_positive (rhs) with
-    | POSITIVE_XH =>
-      v_HaxInt_ZERO
-    | POSITIVE_XO (q)
-    | POSITIVE_XI (q) =>
+  end.
+
+Definition haxint_sub__double_pred_mask (lhs : Core_Base_Spec_Binary_Positive.t_Positive) : t_Mask :=
+  match Core_Base_Spec_Binary_Positive.match_positive (lhs) with
+  | Core_Base_Spec_Binary_Positive.POSITIVE_XH =>
+    Mask_IsNul
+  | Core_Base_Spec_Binary_Positive.POSITIVE_XO (p) =>
+    Mask_IsPos (Core_Base_Spec_Binary_Positive.xO (Core_Base_Binary.positive_pred_double (p)))
+  | Core_Base_Spec_Binary_Positive.POSITIVE_XI (p) =>
+    Mask_IsPos (Core_Base_Spec_Binary_Positive.xO (Core_Base_Spec_Binary_Positive.xO (p)))
+  end.
+
+Definition haxint_sub__succ_double_mask (lhs : t_Mask) : t_Mask :=
+  match lhs with
+  | Mask_IsNeg =>
+    Mask_IsNeg
+  | Mask_IsNul =>
+    Mask_IsPos (Core_Base_Spec_Binary_Positive.xH)
+  | Mask_IsPos (p) =>
+    Mask_IsPos (Core_Base_Spec_Binary_Positive.xI (p))
+  end.
+
+Definition haxint_sub__double_mask (lhs : t_Mask) : t_Mask :=
+  match lhs with
+  | Mask_IsNeg =>
+    Mask_IsNeg
+  | Mask_IsNul =>
+    Mask_IsNul
+  | Mask_IsPos (p) =>
+    Mask_IsPos (Core_Base_Spec_Binary_Positive.xO (p))
+  end.
+
+Definition haxint_double (s : Core_Base_Spec_Haxint.t_HaxInt) : Core_Base_Spec_Haxint.t_HaxInt :=
+  match Core_Base_Spec_Binary_Pos.match_pos (s) with
+  | Core_Base_Spec_Binary_Pos.POS_ZERO =>
+    Core_Base_Spec_Haxint.v_HaxInt_ZERO
+  | Core_Base_Spec_Binary_Pos.POS_POS (p) =>
+    Core_Base_Spec_Binary_Positive.positive_to_int (Core_Base_Spec_Binary_Positive.xO (p))
+  end.
+
+Definition haxint_succ_double (s : Core_Base_Spec_Haxint.t_HaxInt) : Core_Base_Spec_Binary_Positive.t_Positive :=
+  match Core_Base_Spec_Binary_Pos.match_pos (s) with
+  | Core_Base_Spec_Binary_Pos.POS_ZERO =>
+    Core_Base_Spec_Binary_Positive.xH
+  | Core_Base_Spec_Binary_Pos.POS_POS (p) =>
+    Core_Base_Spec_Binary_Positive.xI (p)
+  end.
+
+Definition haxint_mul (lhs : Core_Base_Spec_Haxint.t_HaxInt) (rhs : Core_Base_Spec_Haxint.t_HaxInt) : Core_Base_Spec_Haxint.t_HaxInt :=
+  match Core_Base_Spec_Binary_Pos.match_pos (lhs) with
+  | Core_Base_Spec_Binary_Pos.POS_ZERO =>
+    Core_Base_Spec_Haxint.v_HaxInt_ZERO
+  | Core_Base_Spec_Binary_Pos.POS_POS (p) =>
+    match Core_Base_Spec_Binary_Pos.match_pos (rhs) with
+    | Core_Base_Spec_Binary_Pos.POS_ZERO =>
+      Core_Base_Spec_Haxint.v_HaxInt_ZERO
+    | Core_Base_Spec_Binary_Pos.POS_POS (q) =>
+      Core_Base_Spec_Binary_Positive.positive_to_int (Core_Base_Binary.positive_mul (p) (q))
+    end
+  end.
+
+Definition haxint_shr__half (s : Core_Base_Spec_Haxint.t_HaxInt) : Core_Base_Spec_Haxint.t_HaxInt :=
+  match Core_Base_Spec_Binary_Pos.match_pos (s) with
+  | Core_Base_Spec_Binary_Pos.POS_ZERO =>
+    Core_Base_Spec_Haxint.v_HaxInt_ZERO
+  | Core_Base_Spec_Binary_Pos.POS_POS (n) =>
+    match Core_Base_Spec_Binary_Positive.match_positive (n) with
+    | Core_Base_Spec_Binary_Positive.POSITIVE_XH =>
+      Core_Base_Spec_Haxint.v_HaxInt_ZERO
+    | Core_Base_Spec_Binary_Positive.POSITIVE_XO (p) =>
+      Core_Base_Spec_Binary_Positive.positive_to_int (p)
+    | Core_Base_Spec_Binary_Positive.POSITIVE_XI (p) =>
+      Core_Base_Spec_Binary_Positive.positive_to_int (p)
+    end
+  end.
+
+Definition haxint_sub (lhs : Core_Base_Spec_Haxint.t_HaxInt) (rhs : Core_Base_Spec_Haxint.t_HaxInt) : Core_Base_Spec_Haxint.t_HaxInt :=
+  match Core_Base_Spec_Binary_Pos.match_pos (lhs) with
+  | Core_Base_Spec_Binary_Pos.POS_ZERO =>
+    Core_Base_Spec_Haxint.v_HaxInt_ZERO
+  | Core_Base_Spec_Binary_Pos.POS_POS (p) =>
+    match Core_Base_Spec_Binary_Pos.match_pos (rhs) with
+    | Core_Base_Spec_Binary_Pos.POS_ZERO =>
+      Core_Base_Spec_Binary_Positive.positive_to_int (p)
+    | Core_Base_Spec_Binary_Pos.POS_POS (q) =>
+      match haxint_sub__sub_binary (p) (q) with
+      | Mask_IsPos (v) =>
+        Core_Base_Spec_Binary_Positive.positive_to_int (v)
+      | _ =>
+        Core_Base_Spec_Haxint.v_HaxInt_ZERO
+      end
+    end
+  end.
+
+Fixpoint power_of_two (s : Core_Base_Spec_Unary.t_Unary) : Core_Base_Spec_Binary_Positive.t_Positive :=
+  match Core_Base_Spec_Unary.match_unary (s) with
+  | Core_Base_Spec_Unary.UNARY_ZERO =>
+    Core_Base_Spec_Binary_Positive.xH
+  | Core_Base_Spec_Unary.UNARY_SUCC (x) =>
+    Core_Base_Spec_Binary_Positive.xO (power_of_two (x))
+  end.
+
+Fixpoint haxint_shl__shl_helper (rhs : Core_Base_Spec_Unary.t_Unary) (lhs : Core_Base_Spec_Haxint.t_HaxInt) : Core_Base_Spec_Haxint.t_HaxInt :=
+  if
+    Core_Base_Spec_Haxint.is_zero (Core_Clone.Clone__f_clone (lhs))
+  then
+    lhs
+  else
+    match Core_Base_Spec_Unary.match_unary (rhs) with
+    | Core_Base_Spec_Unary.UNARY_ZERO =>
+      lhs
+    | Core_Base_Spec_Unary.UNARY_SUCC (n) =>
+      haxint_shl__shl_helper (n) (haxint_double (lhs))
+    end.
+
+Fixpoint haxint_shr__shr_helper (rhs : Core_Base_Spec_Unary.t_Unary) (lhs : Core_Base_Spec_Haxint.t_HaxInt) : Core_Base_Spec_Haxint.t_HaxInt :=
+  if
+    Core_Base_Spec_Haxint.is_zero (Core_Clone.Clone__f_clone (lhs))
+  then
+    lhs
+  else
+    match Core_Base_Spec_Unary.match_unary (rhs) with
+    | Core_Base_Spec_Unary.UNARY_ZERO =>
+      lhs
+    | Core_Base_Spec_Unary.UNARY_SUCC (n) =>
+      haxint_shr__shr_helper (n) (haxint_shr__half (lhs))
+    end.
+
+Fixpoint bitxor_binary (lhs : Core_Base_Spec_Binary_Positive.t_Positive) (rhs : Core_Base_Spec_Binary_Positive.t_Positive) : Core_Base_Spec_Haxint.t_HaxInt :=
+  match Core_Base_Spec_Binary_Positive.match_positive (lhs) with
+  | Core_Base_Spec_Binary_Positive.POSITIVE_XH =>
+    match Core_Base_Spec_Binary_Positive.match_positive (rhs) with
+    | Core_Base_Spec_Binary_Positive.POSITIVE_XH =>
+      Core_Base_Spec_Haxint.v_HaxInt_ZERO
+    | Core_Base_Spec_Binary_Positive.POSITIVE_XO (q) =>
+      Core_Base_Spec_Binary_Positive.positive_to_int (Core_Base_Spec_Binary_Positive.xI (q))
+    | Core_Base_Spec_Binary_Positive.POSITIVE_XI (q) =>
+      Core_Base_Spec_Binary_Positive.positive_to_int (Core_Base_Spec_Binary_Positive.xO (q))
+    end
+  | Core_Base_Spec_Binary_Positive.POSITIVE_XO (p) =>
+    match Core_Base_Spec_Binary_Positive.match_positive (rhs) with
+    | Core_Base_Spec_Binary_Positive.POSITIVE_XH =>
+      Core_Base_Spec_Binary_Positive.positive_to_int (Core_Base_Spec_Binary_Positive.xI (p))
+    | Core_Base_Spec_Binary_Positive.POSITIVE_XO (q) =>
+      haxint_double (bitxor_binary (p) (q))
+    | Core_Base_Spec_Binary_Positive.POSITIVE_XI (q) =>
+      Core_Base_Spec_Binary_Positive.positive_to_int (haxint_succ_double (bitxor_binary (p) (q)))
+    end
+  | Core_Base_Spec_Binary_Positive.POSITIVE_XI (p) =>
+    match Core_Base_Spec_Binary_Positive.match_positive (rhs) with
+    | Core_Base_Spec_Binary_Positive.POSITIVE_XH =>
+      Core_Base_Spec_Binary_Positive.positive_to_int (Core_Base_Spec_Binary_Positive.xO (p))
+    | Core_Base_Spec_Binary_Positive.POSITIVE_XO (q) =>
+      Core_Base_Spec_Binary_Positive.positive_to_int (haxint_succ_double (bitxor_binary (p) (q)))
+    | Core_Base_Spec_Binary_Positive.POSITIVE_XI (q) =>
+      haxint_double (bitxor_binary (p) (q))
+    end
+  end.
+
+Fixpoint bitand_binary (lhs : Core_Base_Spec_Binary_Positive.t_Positive) (rhs : Core_Base_Spec_Binary_Positive.t_Positive) : Core_Base_Spec_Haxint.t_HaxInt :=
+  match Core_Base_Spec_Binary_Positive.match_positive (lhs) with
+  | Core_Base_Spec_Binary_Positive.POSITIVE_XH =>
+    match Core_Base_Spec_Binary_Positive.match_positive (rhs) with
+    | Core_Base_Spec_Binary_Positive.POSITIVE_XO (q) =>
+      Core_Base_Spec_Haxint.v_HaxInt_ZERO
+    | Core_Base_Spec_Binary_Positive.POSITIVE_XI (_)
+    | Core_Base_Spec_Binary_Positive.POSITIVE_XH =>
+      Core_Base_Spec_Haxint.v_HaxInt_ONE
+    end
+  | Core_Base_Spec_Binary_Positive.POSITIVE_XO (p) =>
+    match Core_Base_Spec_Binary_Positive.match_positive (rhs) with
+    | Core_Base_Spec_Binary_Positive.POSITIVE_XH =>
+      Core_Base_Spec_Haxint.v_HaxInt_ZERO
+    | Core_Base_Spec_Binary_Positive.POSITIVE_XO (q)
+    | Core_Base_Spec_Binary_Positive.POSITIVE_XI (q) =>
       haxint_double (bitand_binary (p) (q))
     end
-  | POSITIVE_XI (p) =>
-    match match_positive (rhs) with
-    | POSITIVE_XH =>
-      v_HaxInt_ONE
-    | POSITIVE_XO (q) =>
+  | Core_Base_Spec_Binary_Positive.POSITIVE_XI (p) =>
+    match Core_Base_Spec_Binary_Positive.match_positive (rhs) with
+    | Core_Base_Spec_Binary_Positive.POSITIVE_XH =>
+      Core_Base_Spec_Haxint.v_HaxInt_ONE
+    | Core_Base_Spec_Binary_Positive.POSITIVE_XO (q) =>
       haxint_double (bitand_binary (p) (q))
-    | POSITIVE_XI (q) =>
-      positive_to_int (haxint_succ_double (bitand_binary (p) (q)))
+    | Core_Base_Spec_Binary_Positive.POSITIVE_XI (q) =>
+      Core_Base_Spec_Binary_Positive.positive_to_int (haxint_succ_double (bitand_binary (p) (q)))
     end
   end.
 
-Fixpoint bitor_binary (lhs : t_Positive) (rhs : t_Positive) : t_Positive :=
-  match match_positive (lhs) with
-  | POSITIVE_XH =>
-    match match_positive (rhs) with
-    | POSITIVE_XO (q) =>
-      xI (q)
-    | POSITIVE_XH =>
-      xH
-    | POSITIVE_XI (q) =>
-      xI (q)
+Fixpoint bitor_binary (lhs : Core_Base_Spec_Binary_Positive.t_Positive) (rhs : Core_Base_Spec_Binary_Positive.t_Positive) : Core_Base_Spec_Binary_Positive.t_Positive :=
+  match Core_Base_Spec_Binary_Positive.match_positive (lhs) with
+  | Core_Base_Spec_Binary_Positive.POSITIVE_XH =>
+    match Core_Base_Spec_Binary_Positive.match_positive (rhs) with
+    | Core_Base_Spec_Binary_Positive.POSITIVE_XO (q) =>
+      Core_Base_Spec_Binary_Positive.xI (q)
+    | Core_Base_Spec_Binary_Positive.POSITIVE_XH =>
+      Core_Base_Spec_Binary_Positive.xH
+    | Core_Base_Spec_Binary_Positive.POSITIVE_XI (q) =>
+      Core_Base_Spec_Binary_Positive.xI (q)
     end
-  | POSITIVE_XO (p) =>
-    match match_positive (rhs) with
-    | POSITIVE_XH =>
-      xI (p)
-    | POSITIVE_XO (q) =>
-      xO (bitor_binary (p) (q))
-    | POSITIVE_XI (q) =>
-      xI (bitor_binary (p) (q))
+  | Core_Base_Spec_Binary_Positive.POSITIVE_XO (p) =>
+    match Core_Base_Spec_Binary_Positive.match_positive (rhs) with
+    | Core_Base_Spec_Binary_Positive.POSITIVE_XH =>
+      Core_Base_Spec_Binary_Positive.xI (p)
+    | Core_Base_Spec_Binary_Positive.POSITIVE_XO (q) =>
+      Core_Base_Spec_Binary_Positive.xO (bitor_binary (p) (q))
+    | Core_Base_Spec_Binary_Positive.POSITIVE_XI (q) =>
+      Core_Base_Spec_Binary_Positive.xI (bitor_binary (p) (q))
     end
-  | POSITIVE_XI (p) =>
-    match match_positive (rhs) with
-    | POSITIVE_XH =>
-      xI (p)
-    | POSITIVE_XO (q)
-    | POSITIVE_XI (q) =>
-      xI (bitor_binary (p) (q))
+  | Core_Base_Spec_Binary_Positive.POSITIVE_XI (p) =>
+    match Core_Base_Spec_Binary_Positive.match_positive (rhs) with
+    | Core_Base_Spec_Binary_Positive.POSITIVE_XH =>
+      Core_Base_Spec_Binary_Positive.xI (p)
+    | Core_Base_Spec_Binary_Positive.POSITIVE_XO (q)
+    | Core_Base_Spec_Binary_Positive.POSITIVE_XI (q) =>
+      Core_Base_Spec_Binary_Positive.xI (bitor_binary (p) (q))
     end
   end.
 
-Definition haxint_bitand (lhs : t_HaxInt) (rhs : t_HaxInt) : t_HaxInt :=
-  match match_pos (lhs) with
-  | POS_ZERO =>
-    v_HaxInt_ZERO
-  | POS_POS (p) =>
-    match match_pos (rhs) with
-    | POS_ZERO =>
-      v_HaxInt_ZERO
-    | POS_POS (q) =>
+Definition haxint_shl (lhs : Core_Base_Spec_Haxint.t_HaxInt) (rhs : Core_Base_Spec_Haxint.t_HaxInt) : Core_Base_Spec_Haxint.t_HaxInt :=
+  haxint_shl__shl_helper (Core_Base_Spec_Unary.unary_from_int (rhs)) (lhs).
+
+Definition haxint_shr (lhs : Core_Base_Spec_Haxint.t_HaxInt) (rhs : Core_Base_Spec_Haxint.t_HaxInt) : Core_Base_Spec_Haxint.t_HaxInt :=
+  haxint_shr__shr_helper (Core_Base_Spec_Unary.unary_from_int (rhs)) (lhs).
+
+Definition haxint_bitxor (lhs : Core_Base_Spec_Haxint.t_HaxInt) (rhs : Core_Base_Spec_Haxint.t_HaxInt) : Core_Base_Spec_Haxint.t_HaxInt :=
+  match Core_Base_Spec_Binary_Pos.match_pos (lhs) with
+  | Core_Base_Spec_Binary_Pos.POS_ZERO =>
+    rhs
+  | Core_Base_Spec_Binary_Pos.POS_POS (p) =>
+    match Core_Base_Spec_Binary_Pos.match_pos (rhs) with
+    | Core_Base_Spec_Binary_Pos.POS_ZERO =>
+      Core_Base_Spec_Binary_Positive.positive_to_int (p)
+    | Core_Base_Spec_Binary_Pos.POS_POS (q) =>
+      bitxor_binary (p) (q)
+    end
+  end.
+
+Definition haxint_bitand (lhs : Core_Base_Spec_Haxint.t_HaxInt) (rhs : Core_Base_Spec_Haxint.t_HaxInt) : Core_Base_Spec_Haxint.t_HaxInt :=
+  match Core_Base_Spec_Binary_Pos.match_pos (lhs) with
+  | Core_Base_Spec_Binary_Pos.POS_ZERO =>
+    Core_Base_Spec_Haxint.v_HaxInt_ZERO
+  | Core_Base_Spec_Binary_Pos.POS_POS (p) =>
+    match Core_Base_Spec_Binary_Pos.match_pos (rhs) with
+    | Core_Base_Spec_Binary_Pos.POS_ZERO =>
+      Core_Base_Spec_Haxint.v_HaxInt_ZERO
+    | Core_Base_Spec_Binary_Pos.POS_POS (q) =>
       bitand_binary (p) (q)
     end
   end.
 
-Definition haxint_bitor (lhs : t_HaxInt) (rhs : t_HaxInt) : t_HaxInt :=
-  match match_pos (lhs) with
-  | POS_ZERO =>
+Definition haxint_bitor (lhs : Core_Base_Spec_Haxint.t_HaxInt) (rhs : Core_Base_Spec_Haxint.t_HaxInt) : Core_Base_Spec_Haxint.t_HaxInt :=
+  match Core_Base_Spec_Binary_Pos.match_pos (lhs) with
+  | Core_Base_Spec_Binary_Pos.POS_ZERO =>
     rhs
-  | POS_POS (p) =>
-    match match_pos (rhs) with
-    | POS_ZERO =>
-      positive_to_int (p)
-    | POS_POS (q) =>
-      positive_to_int (bitor_binary (p) (q))
+  | Core_Base_Spec_Binary_Pos.POS_POS (p) =>
+    match Core_Base_Spec_Binary_Pos.match_pos (rhs) with
+    | Core_Base_Spec_Binary_Pos.POS_ZERO =>
+      Core_Base_Spec_Binary_Positive.positive_to_int (p)
+    | Core_Base_Spec_Binary_Pos.POS_POS (q) =>
+      Core_Base_Spec_Binary_Positive.positive_to_int (bitor_binary (p) (q))
     end
   end.
 
-Fixpoint haxint_bitxor__bitxor_binary (lhs : t_Positive) (rhs : t_Positive) : t_HaxInt :=
-  match match_positive (lhs) with
-  | POSITIVE_XH =>
-    match match_positive (rhs) with
-    | POSITIVE_XH =>
-      v_HaxInt_ZERO
-    | POSITIVE_XO (q) =>
-      positive_to_int (xI (q))
-    | POSITIVE_XI (q) =>
-      positive_to_int (xO (q))
+Fixpoint haxint_divmod__divmod_binary (a : Core_Base_Spec_Binary_Positive.t_Positive) (b : Core_Base_Spec_Binary_Positive.t_Positive) : (Core_Base_Spec_Haxint.t_HaxInt*Core_Base_Spec_Haxint.t_HaxInt) :=
+  match Core_Base_Spec_Binary_Positive.match_positive (a) with
+  | Core_Base_Spec_Binary_Positive.POSITIVE_XH =>
+    match Core_Base_Spec_Binary_Positive.match_positive (b) with
+    | Core_Base_Spec_Binary_Positive.POSITIVE_XH =>
+      (Core_Base_Spec_Haxint.v_HaxInt_ONE,Core_Base_Spec_Haxint.v_HaxInt_ZERO)
+    | Core_Base_Spec_Binary_Positive.POSITIVE_XO (q)
+    | Core_Base_Spec_Binary_Positive.POSITIVE_XI (q) =>
+      (Core_Base_Spec_Haxint.v_HaxInt_ZERO,Core_Base_Spec_Haxint.v_HaxInt_ONE)
     end
-  | POSITIVE_XO (p) =>
-    match match_positive (rhs) with
-    | POSITIVE_XH =>
-      positive_to_int (xI (p))
-    | POSITIVE_XO (q) =>
-      haxint_double (haxint_bitxor__bitxor_binary (p) (q))
-    | POSITIVE_XI (q) =>
-      positive_to_int (haxint_succ_double (haxint_bitxor__bitxor_binary (p) (q)))
-    end
-  | POSITIVE_XI (p) =>
-    match match_positive (rhs) with
-    | POSITIVE_XH =>
-      positive_to_int (xO (p))
-    | POSITIVE_XO (q) =>
-      positive_to_int (haxint_succ_double (haxint_bitxor__bitxor_binary (p) (q)))
-    | POSITIVE_XI (q) =>
-      haxint_double (haxint_bitxor__bitxor_binary (p) (q))
-    end
-  end.
-
-Definition haxint_bitxor (lhs : t_HaxInt) (rhs : t_HaxInt) : t_HaxInt :=
-  match match_pos (lhs) with
-  | POS_ZERO =>
-    rhs
-  | POS_POS (p) =>
-    match match_pos (rhs) with
-    | POS_ZERO =>
-      positive_to_int (p)
-    | POS_POS (q) =>
-      haxint_bitxor__bitxor_binary (p) (q)
-    end
-  end.
-
-Definition haxint_cmp (lhs : t_HaxInt) (rhs : t_HaxInt) : t_Ordering :=
-  match match_pos (lhs) with
-  | POS_ZERO =>
-    match match_pos (rhs) with
-    | POS_ZERO =>
-      Ordering_Equal
-    | POS_POS (q) =>
-      Ordering_Less
-    end
-  | POS_POS (p) =>
-    match match_pos (rhs) with
-    | POS_ZERO =>
-      Ordering_Greater
-    | POS_POS (q) =>
-      positive_cmp (p) (q)
-    end
-  end.
-
-Definition haxint_le (lhs : t_HaxInt) (rhs : t_HaxInt) : bool :=
-  match Option_Some (haxint_cmp (lhs) (rhs)) with
-  | Option_Some (Ordering_Less
-  | Ordering_Equal) =>
-    true
-  | _ =>
-    false
-  end.
-
-Definition haxint_lt (lhs : t_HaxInt) (rhs : t_HaxInt) : bool :=
-  match Option_Some (haxint_cmp (lhs) (rhs)) with
-  | Option_Some (Ordering_Less) =>
-    true
-  | _ =>
-    false
-  end.
-
-Fixpoint haxint_shl__shl_helper (rhs : t_Unary) (lhs : t_HaxInt) : t_HaxInt :=
-  if
-    is_zero (Clone_f_clone (lhs))
-  then
-    lhs
-  else
-    match match_unary (rhs) with
-    | UNARY_ZERO =>
-      lhs
-    | UNARY_SUCC (n) =>
-      haxint_shl__shl_helper (n) (haxint_double (lhs))
-    end.
-
-Definition haxint_shl (lhs : t_HaxInt) (rhs : t_HaxInt) : t_HaxInt :=
-  haxint_shl__shl_helper (unary_from_int (rhs)) (lhs).
-
-Fixpoint haxint_shr__shr_helper (rhs : t_Unary) (lhs : t_HaxInt) : t_HaxInt :=
-  if
-    is_zero (Clone_f_clone (lhs))
-  then
-    lhs
-  else
-    match match_unary (rhs) with
-    | UNARY_ZERO =>
-      lhs
-    | UNARY_SUCC (n) =>
-      haxint_shr__shr_helper (n) (haxint_shr__half (lhs))
-    end.
-
-Definition haxint_shr (lhs : t_HaxInt) (rhs : t_HaxInt) : t_HaxInt :=
-  haxint_shr__shr_helper (unary_from_int (rhs)) (lhs).
-
-Definition haxint_sub__double_pred_mask (lhs : t_Positive) : t_HaxInt :=
-  match match_positive (lhs) with
-  | POSITIVE_XH =>
-    v_HaxInt_ZERO
-  | POSITIVE_XO (p) =>
-    positive_to_int (xO (positive_pred_double (p)))
-  | POSITIVE_XI (p) =>
-    positive_to_int (xO (xO (p)))
-  end.
-
-Fixpoint power_of_two (s : t_Unary) : t_Positive :=
-  match match_unary (s) with
-  | UNARY_ZERO =>
-    xH
-  | UNARY_SUCC (x) =>
-    xO (power_of_two (x))
-  end.
-
-Definition haxint_add (lhs : t_HaxInt) (rhs : t_HaxInt) : t_HaxInt :=
-  match match_pos (lhs) with
-  | POS_ZERO =>
-    rhs
-  | POS_POS (p) =>
-    match match_pos (rhs) with
-    | POS_ZERO =>
-      positive_to_int (p)
-    | POS_POS (q) =>
-      positive_to_int (positive_add (p) (q))
-    end
-  end.
-
-Fixpoint haxint_sub__sub_binary (lhs : t_Positive) (rhs : t_Positive) : t_HaxInt :=
-  match match_positive (lhs) with
-  | POSITIVE_XH =>
-    v_HaxInt_ZERO
-  | POSITIVE_XO (p) =>
-    match match_positive (rhs) with
-    | POSITIVE_XH =>
-      positive_to_int (positive_pred_double (p))
-    | POSITIVE_XO (q) =>
-      haxint_sub__double_mask (haxint_sub__sub_binary (p) (q))
-    | POSITIVE_XI (q) =>
-      haxint_sub__succ_double_mask (haxint_sub__sub_carry (p) (q))
-    end
-  | POSITIVE_XI (p) =>
-    match match_positive (rhs) with
-    | POSITIVE_XH =>
-      positive_to_int (xO (p))
-    | POSITIVE_XO (q) =>
-      haxint_sub__succ_double_mask (haxint_sub__sub_binary (p) (q))
-    | POSITIVE_XI (q) =>
-      haxint_sub__double_mask (haxint_sub__sub_binary (p) (q))
-    end
-  end
-
-with haxint_sub__sub_carry (lhs : t_Positive) (rhs : t_Positive) : t_HaxInt :=
-  match match_positive (lhs) with
-  | POSITIVE_XH =>
-    v_HaxInt_ZERO
-  | POSITIVE_XO (p) =>
-    match match_positive (rhs) with
-    | POSITIVE_XH =>
-      haxint_sub__double_pred_mask (p)
-    | POSITIVE_XO (q) =>
-      haxint_sub__succ_double_mask (haxint_sub__sub_carry (p) (q))
-    | POSITIVE_XI (q) =>
-      haxint_sub__double_mask (haxint_sub__sub_carry (p) (q))
-    end
-  | POSITIVE_XI (p) =>
-    match match_positive (rhs) with
-    | POSITIVE_XH =>
-      positive_to_int (positive_pred_double (p))
-    | POSITIVE_XO (q) =>
-      haxint_sub__double_mask (haxint_sub__sub_binary (p) (q))
-    | POSITIVE_XI (q) =>
-      haxint_sub__succ_double_mask (haxint_sub__sub_carry (p) (q))
-    end
-  end.
-
-Definition haxint_sub (lhs : t_HaxInt) (rhs : t_HaxInt) : t_HaxInt :=
-  match match_pos (lhs) with
-  | POS_ZERO =>
-    v_HaxInt_ZERO
-  | POS_POS (p) =>
-    match match_pos (rhs) with
-    | POS_ZERO =>
-      positive_to_int (p)
-    | POS_POS (q) =>
-      haxint_sub__sub_binary (p) (q)
-    end
-  end.
-
-Fixpoint haxint_divmod__divmod_binary (a : t_Positive) (b : t_Positive) : (t_HaxInt*t_HaxInt) :=
-  match match_positive (a) with
-  | POSITIVE_XH =>
-    match match_positive (b) with
-    | POSITIVE_XH =>
-      (v_HaxInt_ONE,v_HaxInt_ZERO)
-    | POSITIVE_XO (q)
-    | POSITIVE_XI (q) =>
-      (v_HaxInt_ZERO,v_HaxInt_ONE)
-    end
-  | POSITIVE_XO (a___) =>
-    let (q,r) := haxint_divmod__divmod_binary (a___) (Clone_f_clone (b)) in
-    let r___ := haxint_double (r) in
+  | Core_Base_Spec_Binary_Positive.POSITIVE_XO (a_) =>
+    let (q,r) := haxint_divmod__divmod_binary (a_) (Core_Clone.Clone__f_clone (b)) in
+    let r_ := haxint_double (r) in
     if
-      haxint_le (positive_to_int (Clone_f_clone (b))) (Clone_f_clone (r___))
+      haxint_le (Core_Base_Spec_Binary_Positive.positive_to_int (Core_Clone.Clone__f_clone (b))) (Core_Clone.Clone__f_clone (r_))
     then
-      (positive_to_int (haxint_succ_double (q)),haxint_sub (r___) (positive_to_int (b)))
+      (Core_Base_Spec_Binary_Positive.positive_to_int (haxint_succ_double (q)),haxint_sub (r_) (Core_Base_Spec_Binary_Positive.positive_to_int (b)))
     else
-      (haxint_double (q),r___)
-  | POSITIVE_XI (a___) =>
-    let (q,r) := haxint_divmod__divmod_binary (a___) (Clone_f_clone (b)) in
-    let r___ := positive_to_int (haxint_succ_double (r)) in
+      (haxint_double (q),r_)
+  | Core_Base_Spec_Binary_Positive.POSITIVE_XI (a_) =>
+    let (q,r) := haxint_divmod__divmod_binary (a_) (Core_Clone.Clone__f_clone (b)) in
+    let r_ := Core_Base_Spec_Binary_Positive.positive_to_int (haxint_succ_double (r)) in
     if
-      haxint_le (positive_to_int (Clone_f_clone (b))) (Clone_f_clone (r___))
+      haxint_le (Core_Base_Spec_Binary_Positive.positive_to_int (Core_Clone.Clone__f_clone (b))) (Core_Clone.Clone__f_clone (r_))
     then
-      (positive_to_int (haxint_succ_double (q)),haxint_sub (r___) (positive_to_int (b)))
+      (Core_Base_Spec_Binary_Positive.positive_to_int (haxint_succ_double (q)),haxint_sub (r_) (Core_Base_Spec_Binary_Positive.positive_to_int (b)))
     else
-      (haxint_double (q),r___)
+      (haxint_double (q),r_)
   end.
 
-Definition haxint_divmod (a : t_HaxInt) (b : t_HaxInt) : (t_HaxInt*t_HaxInt) :=
-  match match_pos (a) with
-  | POS_ZERO =>
-    (v_HaxInt_ZERO,v_HaxInt_ZERO)
-  | POS_POS (p) =>
-    match match_pos (b) with
-    | POS_ZERO =>
-      (v_HaxInt_ZERO,positive_to_int (p))
-    | POS_POS (q) =>
+Definition haxint_divmod (a : Core_Base_Spec_Haxint.t_HaxInt) (b : Core_Base_Spec_Haxint.t_HaxInt) : (Core_Base_Spec_Haxint.t_HaxInt*Core_Base_Spec_Haxint.t_HaxInt) :=
+  match Core_Base_Spec_Binary_Pos.match_pos (a) with
+  | Core_Base_Spec_Binary_Pos.POS_ZERO =>
+    (Core_Base_Spec_Haxint.v_HaxInt_ZERO,Core_Base_Spec_Haxint.v_HaxInt_ZERO)
+  | Core_Base_Spec_Binary_Pos.POS_POS (p) =>
+    match Core_Base_Spec_Binary_Pos.match_pos (b) with
+    | Core_Base_Spec_Binary_Pos.POS_ZERO =>
+      (Core_Base_Spec_Haxint.v_HaxInt_ZERO,Core_Base_Spec_Binary_Positive.positive_to_int (p))
+    | Core_Base_Spec_Binary_Pos.POS_POS (q) =>
       haxint_divmod__divmod_binary (p) (q)
     end
   end.
 
-Definition haxint_div (lhs : t_HaxInt) (rhs : t_HaxInt) : t_HaxInt :=
+Definition haxint_div (lhs : Core_Base_Spec_Haxint.t_HaxInt) (rhs : Core_Base_Spec_Haxint.t_HaxInt) : Core_Base_Spec_Haxint.t_HaxInt :=
   let (q,_) := haxint_divmod (lhs) (rhs) in
   q.
 
-Definition haxint_mul (lhs : t_HaxInt) (rhs : t_HaxInt) : t_HaxInt :=
-  match match_pos (lhs) with
-  | POS_ZERO =>
-    v_HaxInt_ZERO
-  | POS_POS (p) =>
-    match match_pos (rhs) with
-    | POS_ZERO =>
-      v_HaxInt_ZERO
-    | POS_POS (q) =>
-      positive_to_int (positive_mul (p) (q))
+Definition haxint_rem (lhs : Core_Base_Spec_Haxint.t_HaxInt) (rhs : Core_Base_Spec_Haxint.t_HaxInt) : Core_Base_Spec_Haxint.t_HaxInt :=
+  let (_,r) := haxint_divmod (lhs) (rhs) in
+  r.
+
+Fixpoint haxint_sub__sub_carry (lhs : Core_Base_Spec_Binary_Positive.t_Positive) (rhs : Core_Base_Spec_Binary_Positive.t_Positive) : t_Mask :=
+  match Core_Base_Spec_Binary_Positive.match_positive (lhs) with
+  | Core_Base_Spec_Binary_Positive.POSITIVE_XH =>
+    Mask_IsNeg
+  | Core_Base_Spec_Binary_Positive.POSITIVE_XO (p) =>
+    match Core_Base_Spec_Binary_Positive.match_positive (rhs) with
+    | Core_Base_Spec_Binary_Positive.POSITIVE_XH =>
+      haxint_sub__double_pred_mask (p)
+    | Core_Base_Spec_Binary_Positive.POSITIVE_XO (q) =>
+      haxint_sub__succ_double_mask (haxint_sub__sub_carry (p) (q))
+    | Core_Base_Spec_Binary_Positive.POSITIVE_XI (q) =>
+      haxint_sub__double_mask (haxint_sub__sub_carry (p) (q))
+    end
+  | Core_Base_Spec_Binary_Positive.POSITIVE_XI (p) =>
+    match Core_Base_Spec_Binary_Positive.match_positive (rhs) with
+    | Core_Base_Spec_Binary_Positive.POSITIVE_XH =>
+      Mask_IsPos (Core_Base_Binary.positive_pred_double (p))
+    | Core_Base_Spec_Binary_Positive.POSITIVE_XO (q) =>
+      haxint_sub__double_mask (haxint_sub__sub_binary (p) (q))
+    | Core_Base_Spec_Binary_Positive.POSITIVE_XI (q) =>
+      haxint_sub__succ_double_mask (haxint_sub__sub_carry (p) (q))
     end
   end.
 
-Definition haxint_rem (lhs : t_HaxInt) (rhs : t_HaxInt) : t_HaxInt :=
-  let (_,r) := haxint_divmod (lhs) (rhs) in
-  r.
+Fixpoint haxint_sub__sub_binary (lhs : Core_Base_Spec_Binary_Positive.t_Positive) (rhs : Core_Base_Spec_Binary_Positive.t_Positive) : t_Mask :=
+  match Core_Base_Spec_Binary_Positive.match_positive (lhs) with
+  | Core_Base_Spec_Binary_Positive.POSITIVE_XH =>
+    Mask_IsNeg
+  | Core_Base_Spec_Binary_Positive.POSITIVE_XO (p) =>
+    match Core_Base_Spec_Binary_Positive.match_positive (rhs) with
+    | Core_Base_Spec_Binary_Positive.POSITIVE_XH =>
+      Mask_IsPos (Core_Base_Binary.positive_pred_double (p))
+    | Core_Base_Spec_Binary_Positive.POSITIVE_XO (q) =>
+      haxint_sub__double_mask (haxint_sub__sub_binary (p) (q))
+    | Core_Base_Spec_Binary_Positive.POSITIVE_XI (q) =>
+      haxint_sub__succ_double_mask (haxint_sub__sub_carry (p) (q))
+    end
+  | Core_Base_Spec_Binary_Positive.POSITIVE_XI (p) =>
+    match Core_Base_Spec_Binary_Positive.match_positive (rhs) with
+    | Core_Base_Spec_Binary_Positive.POSITIVE_XH =>
+      Mask_IsPos (Core_Base_Spec_Binary_Positive.xO (p))
+    | Core_Base_Spec_Binary_Positive.POSITIVE_XO (q) =>
+      haxint_sub__succ_double_mask (haxint_sub__sub_binary (p) (q))
+    | Core_Base_Spec_Binary_Positive.POSITIVE_XI (q) =>
+      haxint_sub__double_mask (haxint_sub__sub_binary (p) (q))
+    end
+  end.
