hax-lib/proof-libs/coq/coq/generated-core/src/Core_Convert.v
@@ -9,32 +9,30 @@ Require Import String.
 Require Import Coq.Floats.Floats.
 From RecordUpdate Require Import RecordSet.
 Import RecordSetNotations.
+From Core Require Import Core.
 
-(* From Core Require Import Core. *)
+(* NotImplementedYet *)
 
-From Core Require Import Core_Marker.
-Export Core_Marker.
-
-Class t_From (v_Self : Type) (v_T : Type) (* `{t_Sized (v_Self)} `{t_Sized (v_T)} *) : Type :=
+Class t_Into (v_Self : Type) (v_T : Type) `{Core_Marker.t_Sized (v_Self)} `{Core_Marker.t_Sized (v_T)} : Type :=
   {
-    From_f_from : v_T -> v_Self;
+    Into__f_into : v_Self -> v_T;
   }.
-Arguments t_From (_) (_) (* {_} {_} *).
+Arguments t_Into (_) (_) {_} {_}.
 
-#[global] Instance t_From_46353410 `{v_T : Type} (* `{t_Sized (v_T)} *) : t_From ((v_T)) ((v_T)) :=
+Class t_From (v_Self : Type) (v_T : Type) `{Core_Marker.t_Sized (v_Self)} `{Core_Marker.t_Sized (v_T)} : Type :=
   {
-    From_f_from := fun  (t : v_T)=>
+    From__f_from : v_T -> v_Self;
+  }.
+Arguments t_From (_) (_) {_} {_}.
+
+Instance t_Into_352590089 `{v_T : Type} `{v_U : Type} `{Core_Marker.t_Sized (v_T)} `{Core_Marker.t_Sized (v_U)} `{t_From (v_U) (v_T)} : t_Into ((v_T)) ((v_U)) :=
+  {
+    implaabbcc_t_Into_impl__f_into := fun  (self : v_T)=>
+      From__f_from (self);
+  }.
+
+Instance t_From_581002014 `{v_T : Type} `{Core_Marker.t_Sized (v_T)} : t_From ((v_T)) ((v_T)) :=
+  {
+    implaabbcc_t_From_impl_1__f_from := fun  (t : v_T)=>
       t;
-  }.
-
-Class t_Into (v_Self : Type) (v_T : Type) (* `{t_Sized (v_Self)} `{t_Sized (v_T)} *) : Type :=
-  {
-    Into_f_into : v_Self -> v_T;
-  }.
-Arguments t_Into (_) (_) (* {_} {_} *).
-
-#[global] Instance t_Into_730689925 `{v_T : Type} `{v_U : Type} (* `{t_Sized (v_T)} `{t_Sized (v_U)} *) `{t_From (v_U) (v_T)} : t_Into ((v_T)) ((v_U)) :=
-  {
-    Into_f_into := fun  (self : v_T)=>
-      From_f_from (self);
   }.
