hax-lib/proof-libs/coq/coq/generated-core/src/Core.v
@@ -9,11 +9,10 @@ Require Import String.
 Require Import Coq.Floats.Floats.
 From RecordUpdate Require Import RecordSet.
 Import RecordSetNotations.
-
 (* From Core Require Import Core. *)
 
-From Core Require Import Core_Primitive.
-Export Core_Primitive.
+(* Require Import Core_Marker. *)
+
 
 (* NotImplementedYet *)
 
@@ -25,56 +24,4 @@ Export Core_Primitive.
 
 (* NotImplementedYet *)
 
-(* NotImplementedYet *)
 
-(* NotImplementedYet *)
-
-(* NotImplementedYet *)
-
-(* NotImplementedYet *)
-
-(* NotImplementedYet *)
-
-(* NotImplementedYet *)
-
-(* NotImplementedYet *)
-
-(* NotImplementedYet *)
-
-(* NotImplementedYet *)
-
-(* NotImplementedYet *)
-
-(* NotImplementedYet *)
-
-(* NotImplementedYet *)
-
-(* NotImplementedYet *)
-
-(* NotImplementedYet *)
-
-(* NotImplementedYet *)
-
-(* NotImplementedYet *)
-
-(* NotImplementedYet *)
-
-(* NotImplementedYet *)
-
-From Core Require Import Core_Option.
-Export Core_Option.
-
-From Core Require Import Core_Array_Rec_bundle_579704328.
-Export Core_Array_Rec_bundle_579704328.
-
-From Core Require Import Core_Ops.
-Export Core_Ops.
-
-From Core Require Import Core_Ops_Index.
-Export Core_Ops_Index.
-
-From Core Require Import NumberNotation.
-Export NumberNotation.
-
-From Core Require Import TODO.
-Export TODO.
