hax-lib/proof-libs/coq/coq/generated-core/src/Core_Base_interface.v
@@ -9,15 +9,10 @@ Require Import String.
 Require Import Coq.Floats.Floats.
 From RecordUpdate Require Import RecordSet.
 Import RecordSetNotations.
-
-(* From Core Require Import Core. *)
-
-From Core Require Import Core_Base_interface_Int.
-Export Core_Base_interface_Int.
-
-From Core Require Import Core_Base_interface_Coerce.
-Export Core_Base_interface_Coerce.
+From Core Require Import Core.
 
 (* NotImplementedYet *)
 
-(* NotImplementedYet *)
+
+
+
